theories/iris_system/lib/allocs.v
@@ -4,25 +4,26 @@ From iris.algebra Require Import functions csum excl updates big_op.
 From stdpp Require Import coPset.
 Require Import sflib.
 
-Definition allocsUR (A : cmra) : ucmra :=
-  positive -d> optionUR (csumR (exclR unitO) A).
+Definition allocsUR (K : Type) (A : cmra) : ucmra :=
+  K -d> optionUR (csumR (exclR unitO) A).
 
 (* TODO : SEAL *)
-Definition allocs_auth (A : cmra) (X : coPset) : allocsUR A :=
-  λ γ, if decide (γ ∈ X) then Some (Cinl (Excl tt)) else None.
-Definition allocs_frag {A : cmra} γ a : allocsUR A :=
-  discrete_fun_singleton γ (Some (Cinr a)).
+Definition allocs_auth {K} (A : cmra) (P : K → Prop) `{∀ k, Decision (P k)} : allocsUR K A :=
+  λ k, if decide (P k) then Some (Cinl (Excl tt)) else None.
+Definition allocs_frag `{EqDecision K} {A} k a : allocsUR K A :=
+  discrete_fun_singleton k (Some (Cinr a)).
 Global Instance: Params (@allocs_frag) 4 := {}.
-Global Arguments allocs_frag {_} γ a.
+Global Arguments allocs_frag {_ _ _} k a.
 
 Section allocs.
-  Context `{CmraDiscrete A}.
+  Context `{CmraDiscrete A} `{EqDecision K}.
+  Local Notation allocs_auth := (@allocs_auth K A).
   Implicit Types a b : A.
-  Implicit Types γ : positive.
+  Implicit Types γ : K.
 
-  Global Instance allocs_frag_ne γ : NonExpansive (@allocs_frag A γ).
+  Global Instance allocs_frag_ne γ : NonExpansive (@allocs_frag _ _ A γ).
   Proof. intros n x y eq. apply discrete_fun_singleton_ne. f_equiv. solve_proper. Qed.
-  Global Instance allocs_frag_proper γ : Proper ((≡) ==> (≡)) (@allocs_frag A γ) := ne_proper _.
+  Global Instance allocs_frag_proper γ : Proper ((≡) ==> (≡)) (@allocs_frag _ _ A γ) := ne_proper _.
 
   (** Operation *)
   Lemma allocs_frag_op γ a b : allocs_frag γ a ⋅ allocs_frag γ b ≡ allocs_frag γ (a ⋅ b).
@@ -35,32 +36,36 @@ Section allocs.
   (** Frame-preserving updates *)
   Lemma allocs_frag_update γ a b (UPD : a ~~> b) : allocs_frag γ a ~~> allocs_frag γ b.
   Proof. by apply discrete_fun_singleton_update, option_update, csum_update_r. Qed.
-  (* TODO : This can be further generalized to yielding a set of resources.
-  Refactor when required. *)
-  Lemma allocs_alloc a (X : coPset) (γ : positive) (IN : γ ∈ X) (WF : ✓ a) :
-    allocs_auth A X ~~> allocs_auth A (X ∖ {[γ]}) ⋅ allocs_frag γ a.
+
+  Lemma allocs_alloc a (P Q : K → Prop) γ (WF : ✓ a) `{∀ k, Decision (P k)} `{∀ k, Decision (Q k)}
+      (IMPL : ∀ k, Q k → P k)
+      (DISJ : P γ ∧ ~ Q γ) :
+    allocs_auth P ~~> allocs_auth Q ⋅ allocs_frag γ a.
   Proof.
-    apply discrete_fun_update; intros p; rewrite discrete_fun_lookup_op ?/allocs_auth /allocs_frag.
-    des_ifs.
-    { rewrite discrete_fun_lookup_singleton_ne; ss. set_solver. }
-    { rewrite left_id.
-      destruct (decide (γ = p)); clarify;
-        [rewrite discrete_fun_lookup_singleton | rewrite discrete_fun_lookup_singleton_ne]; ss.
+    eapply discrete_fun_update; intros k; rewrite /allocs_auth /allocs_frag discrete_fun_lookup_op.
+    des_ifs; rewrite ?left_id.
+    { destruct (decide (γ = k)); clarify; des; ss. rewrite discrete_fun_lookup_singleton_ne; ss. }
+    { destruct (decide (γ = k)); clarify;
+        [rewrite discrete_fun_lookup_singleton|rewrite discrete_fun_lookup_singleton_ne]; ss.
       { apply option_update, cmra_update_exclusive; ss. }
-      { rewrite cmra_discrete_total_update.
-        intros [z|]; ss; rewrite left_id -Some_op; intros CONT%exclusive_l; ss.
-        apply Cinl_exclusive; ss.
-      }
+      { eapply cmra_update_included; ss. }
     }
-    { set_solver. }
-    { destruct (decide (γ = p)); clarify.
-      rewrite discrete_fun_lookup_singleton_ne; ss.
-    }
+    { naive_solver. }
+    { destruct (decide (γ = k)); clarify; des; ss. rewrite discrete_fun_lookup_singleton_ne; ss. }
   Qed.
 
-  Lemma allocs_auth_split (X Y Z : coPset) (DISJ : X ∩ Y = ∅) (EQ : Z = X ∪ Y) :
-    allocs_auth A Z ≡ allocs_auth A X ⋅ allocs_auth A Y.
+  Lemma allocs_auth_split (P Q R : K → Prop)
+      `{∀ k, Decision (P k)} `{∀ k, Decision (Q k)} `{∀ k, Decision (R k)}
+      (DISJ : ∀ k, ~ (Q k ∧ R k))
+      (IMPL : ∀ k, Q k ∨ R k → P k) :
+    allocs_auth P ~~> allocs_auth Q ⋅ allocs_auth R.
   Proof.
-    rewrite EQ => x; rewrite discrete_fun_lookup_op /allocs_auth; des_ifs; try set_solver.
+    apply discrete_fun_update; intros p; rewrite discrete_fun_lookup_op ?/allocs_auth /allocs_frag.
+    des_ifs; try (exfalso; eapply DISJ; eauto; fail).
+    { rewrite right_id cmra_discrete_total_update; intros [z|]; ss; rewrite left_id -Some_op.
+      intros ?%exclusive_l; ss; apply Cinl_exclusive; ss.
+    }
+    { hexploit IMPL; eauto; i; ss. }
+    { hexploit IMPL; eauto; i; ss. }
   Qed.
 End allocs.
