examples/incr/IncrHeader.v
@@ -1,5 +1,5 @@
-Require Import CRIS.
+(* Require Import CRIS.
 
 Module IncrName.
   Definition incr := "Incr.incr".
-End IncrName.
+End IncrName. *)
