examples/incr/IncrIAproof.v
@@ -1,21 +1,21 @@
-Require Import CRIS.
+(* Require Import CRIS.
 
-Require Import IncrI IncrA wsim_tactics.
+Require Import IncrI IncrA SchA wsim_tactics wsim_sch.
 
 Module IncrIA. Section IncrIA.
-  Context `{!invG α Σ Γ, !subG Γ Σ, !sinvG Σ Γ α β τ, !MapMGΓ Γ, !memGΓ Γ}.
+  Context `{!invG α Σ Γ, !subG Γ Σ, !sinvG Σ Γ α β τ, !MapMGΓ Γ, !SchAGΣ Σ, !memGΓ Γ}.
 
   Definition Ist : nat → alist key Any.t → alist key Any.t → iProp Σ := λ _ _ _, emp%I.
 
   Context (u_s u_t : univ_id) (n : level).
-  Context (ginv_s : invspec) (spc_s spc_mem : string → option fspec).
+  Context (ginv_s : invspec) (spc_s spc_user_s spc_mem : string → option fspec).
+  Context (SchInSpc : spc_incl (SchAS.spc u_s n spc_user_s) spc_s).
 
   Local Notation MemA := (MemA.t ginv_s spc_mem).
   Local Notation IncrA := (IncrA.t u_s n ginv_s spc_s ★ MemA).
   Local Notation IncrI := (IncrI.t ★ MemA).
   Local Notation IstFull := (IstProd (IstSB IncrA.(HMod.scopes) Ist) IstEq).
 
-  
   Lemma simF_incr : HSim.sim_fun open IncrA IncrI IstFull IncrName.incr.
   Proof.
     init_wsim u_s u_t n.
@@ -24,12 +24,28 @@ Module IncrIA. Section IncrIA.
     iDestruct "ASM" as "[-> ->]". hss. rename q1 into blk, q2 into ofs.
 
     w_steps_l. w_steps_r.
-    prep_l. prep_r.
-    let marker := fresh "MARKER" in
-    set_marker marker;
-    hide_ihyps;
-    hide_itree_r.
-    prep;
-    show_until marker.
+
+    _prep_macro_l; _prep_macro_r.
+    iApply (wsim_yield); first done.
+    iSplitL "IST"; iFrame.
+    clear nths. iIntros (nths st_s st_t) "IST".
+
+    w_steps_r.
+    iApply wsim_reset. iStopProof.
+    revert nths. combine_quant st_s. combine_quant st_t.
+    eapply wsim_coind.
+    iIntros (g' [st_t [st_s nths]]) "IST #MON #CIH /=".
+
+    unfold_iter_r.
+    _prep_macro_r.
+    iApply (wsim_yield); first done.
+    iSplitL "IST"; iFrame.
+    clear nths st_s st_t. iIntros (nths st_s st_t) "IST".
+
+    w_inline_r.
+    w_steps_r.
+    (* TODO : Stuck here *)
+    (* w_force_r () *)
+
   Admitted.
-End IncrIA. End IncrIA.
+End IncrIA. End IncrIA. *)
