examples/incr/IncrMainI.v
@@ -1,0 +1,53 @@
+Require Import CRIS.
+Require Import ImpPrelude IncrMainHeader MemHeader SchHeader.
+
+Module IncrMainI. Section IncrMainI.
+  Context {Σ : GRA}.
+
+  Definition scopes : list string := [].
+
+  Definition main : unit → itree pmodE unit :=
+    λ _,
+      Sch.yield;;;
+      'ptr_raw : val <- ccallU MemName.alloc [Vint 1%Z];;
+      '(blk, ofs) : mblock * ptrofs <- (pargs [Tptr] [ptr_raw])?;;
+      Sch.yield;;;
+      '_ : val <- ccallU MemName.store [Vptr blk ofs; Vint 0%Z];;
+      Sch.yield;;;
+      tid1 <- Sch.spawn ("f", [Vptr blk ofs]↑↑);;
+      Sch.yield;;;
+      tid2 <- Sch.spawn ("f", [Vptr blk ofs]↑↑);;
+      Sch.yield;;;
+      Sch.join unit tid1;;;
+      Sch.yield;;;
+      Sch.join unit tid2;;;
+      Sch.yield;;;
+      'v_raw : val <- ccallU MemName.load [Vptr blk ofs];;
+      'v : Z <- (pargs [Tint] [v_raw])?;;
+      Sch.yield;;;
+      '_ : unit <- trigger (IO "OUT" v);;
+      Ret tt.
+  
+  Definition f : list val → itree pmodE unit :=
+    λ arg,
+      '(blk, ofs) : mblock * ptrofs <- (pargs [Tptr] arg)?;;
+      Sch.yield;;;
+      'v_raw : val <- ccallU MemName.load [Vptr blk ofs];;
+      'v : Z <- (pargs [Tint] [v_raw])?;;
+      '_ : val <- ccallU MemName.store [Vptr blk ofs; Vint (v + 1)%Z];;
+      Ret tt.
+
+  Definition fnsems :=
+    [(MainName.main, (scopes, cfunU main));
+     (MainName.f,    (scopes, cfunU (sfunU f)))].
+
+  Program Definition Mod : PMod.t := {|
+    PMod.scopes := scopes;
+    PMod.fnsems := fnsems;
+    PMod.initial_st := [];
+  |}.
+  Solve All Obligations with prove_scope.
+  Next Obligation. prove_nodup. Qed.
+
+  Definition t : HMod.t := Seal.sealing CRIS (PMod.to_hmod Mod).
+End IncrMainI. End IncrMainI.
