examples/map/MapA.v
@@ -111,30 +111,30 @@ Module MapAS. Section MapAS.
   Qed.
 
   Section spec.
-    Context (υ : univ_id) (n : level).
+    Context (υ : univ_id).
     Definition init_spec : fspec :=
-      w_fspec υ n
+      w_fspec υ
         (fspec_simple
           (λ sz : nat,
             (λ varg, ⌜varg = [Vint sz]↑ ∧ (8 * (Z.of_nat sz) < modulus_64)%Z⌝ ∗ pending,
               λ vret, ⌜vret = Vundef↑⌝ ∗ initial_points_tos sz)))%I.
 
     Definition get_spec: fspec :=
-      w_fspec υ n
+      w_fspec υ
         (fspec_simple
           (λ '(k, v),
             (λ varg, ⌜varg = [Vint k]↑⌝ ∗ points_to k v,
               λ vret, ⌜vret = (Vint v)↑⌝ ∗ points_to k v)))%I.
 
     Definition set_spec: fspec :=
-      w_fspec υ n
+      w_fspec υ
         (fspec_simple
           (λ '(k, w, v),
             (λ varg, ⌜varg = [Vint k; Vint v]↑⌝ ∗ points_to k w,
               λ vret, ⌜vret = Vundef↑⌝ ∗ points_to k v)))%I.
 
     Definition set_by_user_spec: fspec :=
-      w_fspec υ n
+      w_fspec υ
         (fspec_simple
           (λ '(k, w),
             (λ varg, ⌜varg = [Vint k]↑⌝ ∗ points_to k w,
@@ -170,7 +170,7 @@ def set_by_user(k : int) ≡
 
 Module MapA. Section MapA.
   Context `{!invG α Σ Γ, !subG Γ Σ, !sinvG Σ Γ α β τ, !MapMGΓ Γ, !MapAGΓ Γ}.
-  Context (υ : univ_id) (n : level).
+  Context (υ : univ_id).
 
   Definition scopes := ["Map"].
   Definition v_map := "Map" ↯ "map".
@@ -195,10 +195,10 @@ Module MapA. Section MapA.
       ccallN MapName.set [Vint k; Vint v].
 
   Definition fnsems :=
-    [(MapName.init, (scopes, mk_specbody (MapAS.init_spec υ n) fbody_trivial));
-     (MapName.get, (scopes, mk_specbody (MapAS.get_spec υ n) (cfunN get)));
-     (MapName.set, (scopes, mk_specbody (MapAS.set_spec υ n) (cfunN set)));
-     (MapName.set_by_user, (scopes, mk_specbody (MapAS.set_by_user_spec υ n) (cfunN set_by_user)))].
+    [(MapName.init, (scopes, mk_specbody (MapAS.init_spec υ) fbody_trivial));
+     (MapName.get, (scopes, mk_specbody (MapAS.get_spec υ) (cfunN get)));
+     (MapName.set, (scopes, mk_specbody (MapAS.set_spec υ) (cfunN set)));
+     (MapName.set_by_user, (scopes, mk_specbody (MapAS.set_by_user_spec υ) (cfunN set_by_user)))].
 
   Program Definition Mod : SMod.t := {|
     SMod.scopes := scopes;
