examples/map/MapM.v
@@ -16,7 +16,7 @@ Hint Unfold subG_GΓ map_inG : GRA_index.
 
 Module MapMS. Section MapMS.
   Context `{!invG α Σ Γ, !subG Γ Σ, !sinvG Σ Γ α β τ, !MapMGΓ Γ}.
-  Context (υ : univ_id) (n : level).
+  Context (υ : univ_id).
 
   Definition pending : iProp Σ := own base_γ (Excl ()).
   Lemma pending_unique : pending -∗ pending -∗ False.
@@ -26,28 +26,28 @@ Module MapMS. Section MapMS.
   Qed.
 
   Definition init_spec : fspec :=
-    w_fspec υ n
+    w_fspec υ
       (fspec_simple
         (λ (sz : nat),
           (λ varg, ⌜varg = [Vint sz]↑ ∧ (8 * sz < modulus_64)%Z⌝ ∗ pending,
             λ vret, emp)))%I.
 
   Definition get_spec : fspec := 
-    w_fspec υ n
+    w_fspec υ
       (fspec_simple
         (λ k,
           (λ varg, ⌜varg = [Vint k]↑⌝,
             λ vret, emp)))%I.
 
   Definition set_spec : fspec :=
-    w_fspec υ n
+    w_fspec υ
       (fspec_simple
         (λ '(k, v),
           (λ varg, ⌜varg = ([Vint k; Vint v])↑⌝,
             λ vret, emp))%I).
 
   Definition set_by_user_spec : fspec := 
-    w_fspec υ n
+    w_fspec υ
       (fspec_simple
         (λ k,
           (λ varg, ⌜varg = [Vint k]↑⌝,
@@ -84,7 +84,7 @@ def set_by_user(k : int) ≡
 ***)
 Module MapM. Section MapM.
   Context `{!invG α Σ Γ, !subG Γ Σ, !sinvG Σ Γ α β τ, !MapMGΓ Γ}.
-  Context (υ : univ_id) (n : level).
+  Context (υ : univ_id).
 
   Definition scopes := ["Map"].
   Definition v_size := "Map" ↯ "size".
@@ -120,10 +120,10 @@ Module MapM. Section MapM.
       ccallU MapName.set [Vint k; Vint v].
 
   Definition fnsems :=
-    [(MapName.init, (scopes, mk_specbody (MapMS.init_spec υ n) (cfunU init)));
-     (MapName.get, (scopes, mk_specbody (MapMS.get_spec υ n) (cfunU get)));
-     (MapName.set, (scopes, mk_specbody (MapMS.set_spec υ n) (cfunU set)));
-     (MapName.set_by_user, (scopes, mk_specbody (MapMS.set_by_user_spec υ n) (cfunU set_by_user)))].
+    [(MapName.init, (scopes, mk_specbody (MapMS.init_spec υ) (cfunU init)));
+     (MapName.get, (scopes, mk_specbody (MapMS.get_spec υ) (cfunU get)));
+     (MapName.set, (scopes, mk_specbody (MapMS.set_spec υ) (cfunU set)));
+     (MapName.set_by_user, (scopes, mk_specbody (MapMS.set_by_user_spec υ) (cfunU set_by_user)))].
 
   Program Definition Mod : SMod.t := {|
     SMod.scopes := scopes;
